src/Util/Tactics.v
@@ -1,4 +1,18 @@
+Require Import Bool.
+
 Ltac destruct_hypos := repeat (match goal with
   | H : exists a, _ |- _ => destruct H
   | H : ?x /\ ?y |- _ => destruct H
+  | H : ?x && ?y = true |- _ => apply andb_prop in H
   end).
+
+Ltac destruct_if :=
+      match goal with
+        | |- context[if ?X then _ else _] => destruct X eqn:H_eqb
+      end.
+
+Ltac destruct_match :=
+      match goal with
+      | |- context[match ?X with | _ => _ end] => destruct X eqn:?
+      end.
+
